# Problem 6: Sum Square Difference

## Problem

- [Link to the problem](https://projecteuler.net/problem=6)

<div class="problem_content" role="problem">
<p>The sum of the squares of the first ten natural numbers is,</p>
$$1^2 + 2^2 + ... + 10^2 = 385.$$
<p>The square of the sum of the first ten natural numbers is,</p>
$$(1 + 2 + ... + 10)^2 = 55^2 = 3025.$$
<p>Hence the difference between the sum of the squares of the first ten natural numbers and the square of the sum is $3025 - 385 = 2640$.</p>
<p>Find the difference between the sum of the squares of the first one hundred natural numbers and the square of the sum.</p>
</div>

## Notes

We have the following sums:

$$
\begin{align}
\sum_{i=1}^{n} i &= \frac{n(n+1)}{2} \\
\sum_{i=1}^{n} i^2 &= \frac{n(n+1)(2n+1)}{6} \\
\end{align}
$$

We want to find the difference between the square of the sum of the first $n$ integers and the sum of the squares of the first $n$ integers:

$$
\begin{align*}
\left( \sum_{i=1}^{n} i \right)^2 - \sum_{i=1}^{n} i^2 &= \left( \frac{n(n+1)}{2} \right)^2 - \frac{n(n+1)(2n+1)}{6} \\
&= \frac{n^2(n+1)^2}{4} - \frac{n(n+1)(2n+1)}{6} \\
&= \frac{3n^2(n+1)^2 - 2n(n+1)(2n+1)}{12} \\
&= \frac{n(n+1)(3n(n+1) - 2(2n+1))}{12} \\
&= \frac{n(n+1)(3n^2 + 3n - 4n - 2)}{12} \\
&= \frac{n(n+1)(3n^2 - n - 2)}{12} \\
&= \frac{n(n+1)(3n + 2)(n - 1)}{12}
\end{align*}
$$

## Solution

See it on [GitHub](https://github.com/isitreallyalive/euler/blob/main/problems/src/p6.rs).

```rs
{{#include ../../../problems/src/p6.rs}}
```