The fibonacci numbers are $a_0 = 0$, $a_1 = 1$, $a_{n + 2} = a_{n + 1} + a_n$ for $n \geq 0$. We have:

$$
\begin{align*}
a_0 &= 0 && \tag{even} \\
a_1 &= 1 && \tag{odd} \\
a_2 = a_1 + a_0 &= 1 && \tag{odd} \\
a_3 = a_2 + a_1 &= 2 && \tag{even} \\
a_4 = a_3 + a_2 &= 3 && \tag{odd} \\
a_5 = a_4 + a_3 &= 5 && \tag{odd} \\
\end{align*}
$$

**Claim:** For all $k \geq 0$, $a_{3k}$ is even and $a_{3k+1}$, $a_{3k+2}$ are odd.

**Proof by induction:**

**Base case:** $k = 0$
- $a_0 = 0$ (even) ✓
- $a_1 = 1$ (odd) ✓  
- $a_2 = 1$ (odd) ✓

**Inductive step:** Assume the claim holds for some $k \geq 0$. We prove it for $k+1$.

By the inductive hypothesis:
- $a_{3k}$ is even
- $a_{3k+1}$ is odd
- $a_{3k+2}$ is odd

We need to show:
- $a_{3(k+1)} = a_{3k+3}$ is even
- $a_{3(k+1)+1} = a_{3k+4}$ is odd
- $a_{3(k+1)+2} = a_{3k+5}$ is odd

Using the Fibonacci recurrence:

$$a_{3k+3} = a_{3k+2} + a_{3k+1} = \text{odd} + \text{odd} = \text{even}$$

$$a_{3k+4} = a_{3k+3} + a_{3k+2} = \text{even} + \text{odd} = \text{odd}$$

$$a_{3k+5} = a_{3k+4} + a_{3k+3} = \text{odd} + \text{even} = \text{odd}$$

Therefore, the claim holds for $k+1$, completing the induction. $\blacksquare$