We have the following sums:
$$
\begin{align}
\sum_{i=1}^{n} i &= \frac{n(n+1)}{2} \\
\sum_{i=1}^{n} i^2 &= \frac{n(n+1)(2n+1)}{6} \\
\end{align}
$$

We want to find the difference between the square of the sum of the first $n$ integers and the sum of the squares of the first $n$ integers:

$$
\begin{align*}
\left( \sum_{i=1}^{n} i \right)^2 - \sum_{i=1}^{n} i^2 &= \left( \frac{n(n+1)}{2} \right)^2 - \frac{n(n+1)(2n+1)}{6} \\
&= \frac{n^2(n+1)^2}{4} - \frac{n(n+1)(2n+1)}{6} \\
&= \frac{3n^2(n+1)^2 - 2n(n+1)(2n+1)}{12} \\
&= \frac{n(n+1)(3n(n+1) - 2(2n+1))}{12} \\
&= \frac{n(n+1)(3n^2 + 3n - 4n - 2)}{12} \\
&= \frac{n(n+1)(3n^2 - n - 2)}{12} \\
&= \frac{n(n+1)(3n + 2)(n - 1)}{12}
\end{align*}
$$