Let $a$, $b$, and $c$ form a pythagorean triple such that $a + b + c = n$. Then we can manipulate the definition of a pythagorean triple:

$$
\begin{align*}
a^2 + b^2 &= c^2 \\
&= (n - a - b)^2 \\
&= n^2 - 2an - 2bn + a^2 + 2ab + b^2 \\
2an - n^2 &= 2ab - 2bn \\
n(2a - n) &= 2b(a - n) \\
b &= \frac{n(2a - n)}{2(a - n)}
\end{align*}
$$

As such, for a given value $a$, a pythagorean triple with the components summing to $n$ can be constructed by:

$$
\begin{align*}
b = \frac{n(2a - n)}{2(a - n)} && c = n - a - b
\end{align*}
$$